theories/Dot/syn/syn.v
@@ -78,12 +78,6 @@ Fixpoint dms_lookup l ds : option dm :=
     end
   end.
 
-Fixpoint plength p : nat :=
-  match p with
-  | pv _ => 0
-  | pself p _ => S (plength p)
-  end.
-
 Fixpoint path2tm p: tm :=
   match p with
   | pv v => tv v
